proof/uni_counter/algo_worklist/prop_rename.v
@@ -879,59 +879,6 @@ Proof.
 Qed.
 
 
-Lemma rename_tvar_lookup_var_bind_some : forall Γ x X Y A,
-  Y `notin` dom (⌊ Γ ⌋ᵃ) ->
-  lookup_var_bind (⌊ Γ ⌋ᵃ) x = Some A ->
-  lookup_var_bind (⌊ {Y ᵃʷ/ₜᵥ X} Γ ⌋ᵃ ) x = Some ({`Y ᵗ/ₜ X} A).
-Proof.
-  intros. induction Γ; simpl in *; auto.
-  - inversion H0. 
-  - destruct_eq_atom; destruct ab; subst; simpl; destruct_eq_atom; auto; try inversion H0.
-    + subst. auto.
-    + subst. auto.
-Qed.
-
-Lemma rename_tvar_lookup_var_bind_none : forall Γ x X Y,
-  Y `notin` dom (⌊ Γ ⌋ᵃ) ->
-  lookup_var_bind (⌊ Γ ⌋ᵃ) x = None ->
-  lookup_var_bind (⌊ {Y ᵃʷ/ₜᵥ X} Γ ⌋ᵃ ) x = None.
-Proof.
-  intros. induction Γ; simpl in *; auto.
-  destruct_eq_atom; destruct ab; subst; simpl; destruct_eq_atom; auto; try inversion H0.
-Qed.
-
-Lemma rename_tvar_lookup_tvar_bind : forall Γ X' X Y b,
-  b = □ \/ b = ■ \/ b = ⬒ ->
-  Y `notin` dom (⌊ Γ ⌋ᵃ) `union` singleton X' ->
-  lookup_tvar_bind (⌊ Γ ⌋ᵃ) X' = Some b ->
-  lookup_tvar_bind (⌊ {Y ᵃʷ/ₜᵥ X} Γ ⌋ᵃ ) (if X' == X then Y else X' ) = Some b.
-Proof.
-  intros. induction Γ; simpl in *; auto.
-  destruct_eq_atom; destruct ab; subst; simpl; destruct_eq_atom; auto. inversion H1.
-Qed.
-
-Lemma exp_split_size_rename_tvar : forall n e Γ X Y,
-  size_exp e < n -> Y `notin` dom (⌊ Γ ⌋ᵃ) ->
-  exp_split_size (⌊ Γ ⌋ᵃ) e = exp_split_size (⌊ {Y ᵃʷ/ₜᵥ X} Γ ⌋ᵃ) ({` Y ᵉ/ₜ X} e).
-Proof.
-  intro n. induction n; simpl; intros * Hlt Hnotin; try lia.
-  destruct e; simpl in *; auto.
-  - destruct (lookup_var_bind (⌊ Γ ⌋ᵃ) x) eqn:Heq.
-    + erewrite rename_tvar_lookup_var_bind_some; eauto.
-      rewrite <- iuv_size_rename_tvar; auto.
-    + erewrite rename_tvar_lookup_var_bind_none; eauto.
-  - rewrite <- IHn; auto; lia.
-  - repeat rewrite <-IHn; auto; lia.
-  - destruct body5. 
-    simpl in *. repeat rewrite <- IHn; auto. 
-    rewrite <-iuv_size_rename_tvar; auto. lia.
-  - rewrite <- IHn. rewrite <- iuv_size_rename_tvar. auto.
-    lia. auto.
-  - rewrite <- IHn. rewrite <- iuv_size_rename_tvar. auto.
-    lia. auto.
-Qed.
-
-
 Theorem rename_tvar_in_a_wf_wwl_a_wl_red : forall Γ X Y,
   X <> Y ->
   ⊢ᵃʷ Γ ->
@@ -1184,7 +1131,8 @@ Proof with eauto.
       rewrite_env (nil ++ ((X2, ⬒) :: (X1 ~ ⬒)) ++ ⌊ Γ ⌋ᵃ).
       apply a_wf_conts_weaken...
   - simpl in *. destruct_a_wf_wl.
-    constructor. erewrite <- exp_split_size_rename_tvar; eauto.
+    assert (a_exp_split_size (⌊ {Y ᵃʷ/ₜᵥ X} Γ ⌋ᵃ) ({` Y ᵉ/ₜ X} e1) n) by admit.
+    econstructor; eauto.
     eapply IHa_wl_red; eauto.
   - simpl in *. destruct_a_wf_wl. dependent destruction H0.
     inst_cofinites_for a_wl_red__infabs_all.
@@ -1251,7 +1199,7 @@ Proof with eauto.
     eapply a_wl_red__applyd...
     auto_apply...
     eapply a_wf_wwl_apply_contd in H0... 
-Qed.
+Admitted.
 
 
 Theorem rename_tvar_in_a_wf_twl_a_wl_red : forall Γ X Y,
@@ -1796,32 +1744,6 @@ Ltac create_fvar_in_awl_set :=
     assert (Hfv: x ∉ fvar_in_aworklist' Γ) by (rewrite fvar_in_aworklist_upper; auto)
   end.
 
-Lemma rename_var_lookup_var_bind : forall Γ x' x y,
-  y `notin` dom (⌊ Γ ⌋ᵃ) `union` singleton x' ->
-  lookup_var_bind (⌊ Γ ⌋ᵃ) x' = lookup_var_bind (⌊ {y ᵃʷ/ₑᵥ x} Γ ⌋ᵃ ) (if x' == x then y else x').
-Proof.
-  intros. induction Γ; simpl in *; auto; destruct ab; subst; simpl; auto; destruct_eq_atom; auto.
-Qed.
-
-Lemma exp_split_size_rename_var : forall n e Γ x y,
-  size_exp e < n -> y `notin` dom (⌊ Γ ⌋ᵃ) `union` fvar_in_exp e ->
-  exp_split_size (⌊ Γ ⌋ᵃ) e = exp_split_size (⌊ {y ᵃʷ/ₑᵥ x} Γ ⌋ᵃ) ({exp_var_f y ᵉ/ₑ x} e).
-Proof.
-  intro n. induction n; simpl; intros * Hlt Hnotin; try lia.
-  destruct e; simpl in *; auto.
-  - destruct_eq_atom; simpl.
-    + replace (lookup_var_bind (⌊ {y ᵃʷ/ₑᵥ x} Γ ⌋ᵃ) y) with (lookup_var_bind (⌊ {y ᵃʷ/ₑᵥ x} Γ ⌋ᵃ) (if x == x then y else x)).
-      erewrite <- rename_var_lookup_var_bind; eauto. destruct_eq_atom; eauto.
-    + replace (lookup_var_bind (⌊ {y ᵃʷ/ₑᵥ x} Γ ⌋ᵃ) x0) with (lookup_var_bind (⌊ {y ᵃʷ/ₑᵥ x} Γ ⌋ᵃ) (if x0 == x then y else x0)).
-      erewrite <- rename_var_lookup_var_bind; eauto. destruct_eq_atom; eauto.
-  - rewrite <- IHn; auto; lia.
-  - repeat rewrite <-IHn; auto; lia.
-  - destruct body5. 
-    simpl in *. repeat rewrite <- IHn; auto. lia.
-  - rewrite <- IHn; auto. lia.
-  - rewrite <- IHn; auto. lia.
-Qed.
-
 Theorem rename_var_in_a_wf_wwl_a_wl_red : forall Γ x y,
   ⊢ᵃʷ Γ ->
   y <> x ->
@@ -1975,7 +1897,8 @@ Proof with eauto.
     apply a_wf_exp_weaken_etvar_twice with (T:=T)...
     apply a_wf_conts_weaken_cons...  apply a_wf_conts_weaken_cons...
   - simpl in *. destruct_a_wf_wl.
-    constructor. erewrite <- exp_split_size_rename_var; eauto.
+    assert (a_exp_split_size (⌊ {y ᵃʷ/ₑᵥ x} Γ ⌋ᵃ) ({exp_var_f y ᵉ/ₑ x} e1) n) by admit.
+    econstructor; eauto.
     eapply IHa_wl_red; eauto.
   - destruct_a_wf_wl. dependent destruction H. simpl in *.
     inst_cofinites_for a_wl_red__infabs_all.
@@ -2015,7 +1938,7 @@ Proof with eauto.
     econstructor; eauto.
     auto_apply...
     eapply a_wf_wwl_apply_contd; eauto.
-Qed.
+Admitted.
 
 
 Theorem rename_var_in_a_wf_twl_a_wl_red : forall Γ x y,
@@ -2038,5 +1961,5 @@ Theorem rename_var_in_a_wf_wl_a_wl_red : forall Γ x y,
 Proof.
   intros. eapply rename_var_in_a_wf_wwl_a_wl_red; eauto.
   apply a_wf_wl_a_wf_wwl; auto.
-Qed.
+Qed.  
 
